src/lib/kuiper/Kuiper.Kernel.fst
@@ -27,7 +27,50 @@ fn obtain_shmem
   ensures  pure (reveal ear == ar)
     { admit () }
 
+fn sync () (#e:erased nat)
+  requires epoch_live e
+  ensures
+    exists* e'.
+      epoch_live e' ** epoch_done e **
+      pure (e' >= e)
+{ admit (); }
+
+
+fn launch_kernel_n_m_shmem_async
+  (#u1: erased int)
+  (nblk : SZ.t { 0 < nblk /\ nblk <= max_blocks })
+  (nthr : SZ.t { 0 < nthr /\ nthr <= max_threads })
+  (#pre #post : (tid:nat{ 0 <= tid /\ tid < (nblk * nthr) } -> slprop))
+  (a : Type u#0)
+  {| Kuiper.Sized.sized a |}
+  (smem_sz : SZ.t)
+  (#shared_pre : (ar: gpu_array a smem_sz) -> (bid: nat { 0 <= bid /\ bid < nblk }) -> (tid: nat { 0 <= tid /\ tid < nthr } -> slprop))
+  (#shared_post : (ar: gpu_array a smem_sz) -> (bid: nat { 0 <= bid /\ bid < nblk }) -> (tid: nat { 0 <= tid /\ tid < nthr } -> slprop))
+  (setup : (ar: gpu_array a smem_sz) -> (bid: SZ.t { 0 <= bid /\ bid < nblk }) ->
+    stt_ghost unit emp_inames
+      (block_setup nthr ** (exists* v. gpu_pts_to_array #a #smem_sz ar #1.0R v))
+      (fun _ -> block_setup nthr ** bigstar 0 nthr (shared_pre ar bid)))
+
+  (k :
+    (ar: erased (gpu_array a smem_sz)) -> (etid: tid_t { gdim_x etid == nblk /\ bdim_x etid == nthr }) ->
+    stt unit (         gpu ** thread_id etid ** shmem_tok ar ** shared_pre ar (bidx_x etid) (tidx_x etid) ** pre (thread_index etid))
+             (fun _ -> gpu ** thread_id etid **                 shared_post ar (bidx_x etid) (tidx_x etid) ** post (thread_index etid))
+  )
+  (#e : erased nat)
+  requires
+    cpu **
+    epoch_live e **
+    bigstar #u1 0 (nblk * nthr) pre
+  ensures
+    exists* e'.
+      cpu **
+      epoch_live e' **
+      pledge0 (epoch_done e') (bigstar #u1 0 (nblk * nthr) post) **
+      pure (e' >= e)
+{ admit (); }
+
 (* f<<<nblk, nthr, smem_sz>>>(...); *)
+inline_for_extraction
 fn launch_kernel_n_m_shmem
   (#u1: erased int)
   (nblk : SZ.t { 0 < nblk /\ nblk <= max_blocks })
@@ -51,7 +94,17 @@ fn launch_kernel_n_m_shmem
   )
   requires cpu ** bigstar #u1 0 (nblk * nthr) pre
   ensures  cpu ** bigstar #u1 0 (nblk * nthr) post
-{ admit (); }
+{
+  let _ = get_epoch ();
+  launch_kernel_n_m_shmem_async nblk nthr a smem_sz setup k;
+  unfold pledge0;
+  sync ();
+  with e'. assert (epoch_done e');
+  redeem_pledge emp_inames (epoch_done e') _;
+  drop_ (epoch_done e');
+  drop_ (epoch_live _);
+}
+
 
 (* f<<<nblk, nthr>>>(...); *)
 fn launch_kernel_n_m_barrier
@@ -134,30 +187,6 @@ fn kernel_1_as_n
   k ()
 }
 
-let epoch_live (n:nat) : slprop = magic ()
-let epoch_done (n:nat) : slprop = magic ()
-
-ghost
-fn get_epoch ()
-  requires emp
-  returns e : erased nat
-  ensures epoch_live e
-{ admit (); }
-
-fn sync () (#e:erased nat)
-  requires epoch_live e
-  ensures
-    exists* e'.
-      epoch_live e' ** epoch_done e **
-      pure (e' >= e)
-{ admit (); }
-
-ghost
-fn done_lower (e f :nat)
-  requires epoch_done e ** pure (f <= e)
-  ensures  epoch_done e ** epoch_done f
-{ admit (); }
-
 fn launch_kernel_1_async
   (#pre #post : slprop)
   (k : unit ->
@@ -167,22 +196,11 @@ fn launch_kernel_1_async
   requires cpu ** epoch_live e ** pre
   ensures
     exists* e'.
-      cpu ** epoch_live e' ** pledge0 (epoch_done e) post **
+      cpu **
+      epoch_live e' **
+      pledge0 (epoch_done e') post **
       pure (e' >= e)
 { admit (); }
-
-// fn launch_kernel_1
-//   (#pre #post : slprop)
-//   (k : unit ->
-//     stt unit (gpu ** pre) (fun _ -> gpu ** post)
-//   )
-//   requires cpu ** pre
-//   ensures  cpu ** post
-// {
-//   bigstar_single_intro 0 (fun (i: nat { 0 <= i /\ i < 1 }) -> pre);
-//   launch_kernel_n 1sz (fun etid -> kernel_1_as_n #pre #post k etid);
-//   bigstar_single_elim #0;
-// }
 
 inline_for_extraction
 fn launch_kernel_1
