src/lib/kuiper/Kuiper.Epoch.fsti
@@ -1,0 +1,18 @@
+module Kuiper.Epoch
+#lang-pulse
+
+open Pulse
+
+val epoch_live (n:nat) : slprop
+val epoch_done (n:nat) : slprop
+
+ghost
+fn get_epoch ()
+  requires emp
+  returns e : erased nat
+  ensures epoch_live e
+
+ghost
+fn done_lower (e f :nat)
+  requires epoch_done e ** pure (f <= e)
+  ensures  epoch_done e ** epoch_done f
