src/lib/kuiper/Kuiper.Kernel.fsti
@@ -7,6 +7,7 @@ open Kuiper.SizeT
 open Kuiper.Array
 open Kuiper.Base
 open Kuiper.Barrier.RPM
+open Kuiper.Epoch
 open FStar.Mul
 module SZ = FStar.SizeT
 open Pulse.Lib.Pledge
@@ -26,6 +27,45 @@ fn obtain_shmem
   requires shmem_tok ear
   returns  ar : gpu_array a sz
   ensures  pure (reveal ear == ar)
+
+fn sync () (#e:erased nat)
+  requires epoch_live e
+  ensures
+    exists* e'.
+      epoch_live e' ** epoch_done e **
+      pure (e' >= e)
+
+fn launch_kernel_n_m_shmem_async
+  (#u1: erased int)
+  (nblk : SZ.t { 0 < nblk /\ nblk <= max_blocks })
+  (nthr : SZ.t { 0 < nthr /\ nthr <= max_threads })
+  (#pre #post : (tid:nat{ 0 <= tid /\ tid < (nblk * nthr) } -> slprop))
+  (a : Type u#0)
+  {| Kuiper.Sized.sized a |}
+  (smem_sz : SZ.t)
+  (#shared_pre : (ar: gpu_array a smem_sz) -> (bid: nat { 0 <= bid /\ bid < nblk }) -> (tid: nat { 0 <= tid /\ tid < nthr } -> slprop))
+  (#shared_post : (ar: gpu_array a smem_sz) -> (bid: nat { 0 <= bid /\ bid < nblk }) -> (tid: nat { 0 <= tid /\ tid < nthr } -> slprop))
+  (setup : (ar: gpu_array a smem_sz) -> (bid: SZ.t { 0 <= bid /\ bid < nblk }) ->
+    stt_ghost unit emp_inames
+      (block_setup nthr ** (exists* v. gpu_pts_to_array #a #smem_sz ar #1.0R v))
+      (fun _ -> block_setup nthr ** bigstar 0 nthr (shared_pre ar bid)))
+
+  (k :
+    (ar: erased (gpu_array a smem_sz)) -> (etid: tid_t { gdim_x etid == nblk /\ bdim_x etid == nthr }) ->
+    stt unit (         gpu ** thread_id etid ** shmem_tok ar ** shared_pre ar (bidx_x etid) (tidx_x etid) ** pre (thread_index etid))
+             (fun _ -> gpu ** thread_id etid **                 shared_post ar (bidx_x etid) (tidx_x etid) ** post (thread_index etid))
+  )
+  (#e : erased nat)
+  requires
+    cpu **
+    epoch_live e **
+    bigstar #u1 0 (nblk * nthr) pre
+  ensures
+    exists* e'.
+      cpu **
+      epoch_live e' **
+      pledge0 (epoch_done e') (bigstar #u1 0 (nblk * nthr) post) **
+      pure (e' >= e)
 
 (* f<<<nblk, nthr, smem_sz>>>(...); *)
 fn launch_kernel_n_m_shmem
@@ -94,27 +134,6 @@ fn launch_kernel_n
   requires cpu ** bigstar #u1 0 (SZ.v nblk) pre
   ensures  cpu ** bigstar #u1 0 (SZ.v nblk) post
 
-val epoch_live (n:nat) : slprop
-val epoch_done (n:nat) : slprop
-
-ghost
-fn get_epoch ()
-  requires emp
-  returns e : erased nat
-  ensures epoch_live e
-
-fn sync () (#e:erased nat)
-  requires epoch_live e
-  ensures
-    exists* e'.
-      epoch_live e' ** epoch_done e **
-      pure (e' >= e)
-
-ghost
-fn done_lower (e f :nat)
-  requires epoch_done e ** pure (f <= e)
-  ensures  epoch_done e ** epoch_done f
-
 fn launch_kernel_1_async
   (#pre #post : slprop)
   (k : unit ->
@@ -124,7 +143,9 @@ fn launch_kernel_1_async
   requires cpu ** epoch_live e ** pre
   ensures
     exists* e'.
-      cpu ** epoch_live e' ** pledge0 (epoch_done e') post **
+      cpu **
+      epoch_live e' **
+      pledge0 (epoch_done e') post **
       pure (e' >= e)
 
 inline_for_extraction
